formal/Kimchi.lean
@@ -33,5 +33,6 @@ import Kimchi.Circuits.EndoMulStep
 import Kimchi.Circuits.EndoScalarStep
 import Kimchi.Circuits.PoseidonStep
 import Kimchi.Circuits.Combinations
+import Kimchi.Circuits.ScaleCombinePub
 import Kimchi.Circuits.InitGrounding
 import Kimchi.Json
